concrete chat server done except for admitted resdet

abstract_petrinet.v
@@ -1,59 +1,20 @@
-From iris.base_logic Require Import invariants.
+From iris.base_logic Require Import invariants viewshifts.
 From iris.proofmode Require Import tactics.
 From iris_io Require Import petrinet.
 
 Section AbsPetrinet.
   Context `{invG Σ}.
 
-  Class abstract_petrinet :=
-    Abstract_Petrinet {
-        places : Type;
-        token : places → iProp Σ;
-        Split : places → places → places → iProp Σ;
-        Split_pers P Q1 Q2 :> Persistent (Split P Q1 Q2);
-        Split_ws P Q1 Q2 :
-          (Split P Q1 Q2 -∗ token P ={⊤}=∗ token Q1 ∗ token Q2)%I;
-        Join : places → places → places → iProp Σ;
-        Join_pers P1 P2 Q :> Persistent (Join P1 P2 Q);
-        Join_ws P1 P2 Q :
-          (Join P1 P2 Q -∗ token P1 -∗ token P2 ={⊤}=∗ token Q)%I;
-        NoOp : places → places → iProp Σ;
-        NoOp_pers P Q :> Persistent (NoOp P Q);
-        NooP_ws P Q :
-          (NoOp P Q -∗ token P ={⊤}=∗ token Q)%I;
-      }.
+  Definition abs_place := iProp Σ.
+
+  Definition abs_token (P : abs_place) : iProp Σ := P.
+
+  Definition abs_split P Q1 Q2 :=
+    (abs_token P ={⊤}=> abs_token Q1 ∗ abs_token Q2)%I.
+
+  Definition abs_join P1 P2 Q :=
+    (abs_token P1 -∗ abs_token P2 ={⊤}=> abs_token Q)%I.
+
+  Definition abs_noop P Q := (abs_token P ={⊤}=> abs_token Q)%I.
 
 End AbsPetrinet.
-
-Global Arguments places {_ _} _.
-
-Section ConcPetrinet.
-  Context `{heapIG, petrinetIG Σ}.
-
-  Global Program Instance concrete_petrinet : abstract_petrinet :=
-    {|
-      places := Places;
-      token p := Token p;
-      Split p q1 q2 := ⌜ThePetriNet (SplitTr p q1 q2)⌝%I;
-      Join p q1 q2 := ⌜ThePetriNet (JoinTr p q1 q2)⌝%I;
-      NoOp p q := ⌜ThePetriNet (NoOpTr p q)⌝%I;
-    |}.
-
-  Next Obligation.
-  Proof.
-    by iIntros (? ? ? ?) "?"; iApply petrinet_split.
-  Qed.
-
-  Next Obligation.
-  Proof.
-    iIntros (? ? ? ?) "? ?"; iApply petrinet_join; first by eauto.
-    iFrame.
-  Qed.
-
-  Next Obligation.
-  Proof.
-    iIntros (? ? ?) "?"; iApply petrinet_noop; eauto.
-  Qed.
-
-End ConcPetrinet.
-
