chat_server_concrete.v
@@ -1,9 +1,11 @@
 From iris.algebra Require Import auth.
 From iris.proofmode Require Import tactics.
-From iris.base_logic Require Import fixpoint.
+From iris.base_logic Require Import fixpoint viewshifts.
 From iris.program_logic Require Import weakestpre lifting.
 From iris_io Require Import lang rules abstract_petrinet petrinet
      chat_server channel adequacy.
+
+From Coq.Logic Require Import ClassicalDescription.
 
 Section conrete_chat_server.
   Context `{heapIG Σ, petrinetIG Σ, channelIG Σ}.
@@ -11,8 +13,8 @@ Section conrete_chat_server.
   Definition read_nick1 := 1%positive.
   Definition read_nick2 := 2%positive.
 
-  Definition write_nick1 := 1%positive.
-  Definition write_nick2 := 2%positive.
+  Definition write_nick1 := 3%positive.
+  Definition write_nick2 := 4%positive.
 
   Definition bool_to_write_tag (b : bool) :=
     if b then write_nick1 else write_nick2.
@@ -91,30 +93,35 @@ Section conrete_chat_server.
     uPred_greatest_fixpoint (IO_pre_sequence io_gen).
 
   Definition ReceiveFromNick :=
-    λ p n μ,
+    λ P n μ,
     match n with
     | BoolV b =>
-      (IO_sequence (λ v p q, IOTr p (bool_to_read_tag b) UnitV v q) (p, μ))%I
+      (∃ p, (P ={⊤}=> Token p)
+              ∗ IO_sequence (λ v p q, IOTr p (bool_to_read_tag b) UnitV v q)
+              (p, μ))%I
     | _ => False%I
     end.
 
   Definition SendToNick :=
-    λ p n μ,
+    λ P n μ,
     match n with
     | BoolV b =>
-      (IO_sequence (λ v p q, IOTr p (bool_to_write_tag b) v UnitV q) (p, μ))%I
+      (∃ p, (P ={⊤}=> Token p)
+              ∗ IO_sequence (λ v p q, IOTr p (bool_to_write_tag b) v UnitV q) (p, μ))%I
     | _ => False%I
     end.
 
-  Lemma wp_receive_from_nick : ∀ r n m μ,
-    {{{ token r ∗ ReceiveFromNick r n {| Shead := m; Stail := μ|} }}}
+  Lemma wp_receive_from_nick : ∀ P n m μ,
+    {{{ P ∗ ReceiveFromNick P n {| Shead := m; Stail := μ|} }}}
       App receive_from_nick (of_val n)
-    {{{ RET m; ∃ r', token r' ∗ ReceiveFromNick r' n μ }}}.
+    {{{ RET m; ∃ Q, Q ∗ ReceiveFromNick Q n μ }}}.
   Proof.
-    iIntros (r n m μ Φ) "[Hr Hrfn] HΦ".
+    iIntros (P n m μ Φ) "[Hr Hrfn] HΦ".
     iApply wp_pure_step_later; trivial.
     iNext. asimpl.
     destruct n; simpl; try done.
+    iDestruct "Hrfn" as (r) "[#HPr Hrfn]".
+    iMod ("HPr" with "Hr") as "Hr".
     rewrite {1}/IO_sequence greatest_fixpoint_unfold.
     iDestruct "Hrfn" as (q) "/= [% Hrfn]".
     iApply (wp_bind (fill [IOLCtx _])).
@@ -122,32 +129,37 @@ Section conrete_chat_server.
     iNext; iIntros "_"; simpl.
     iApply (wp_petrinet_io with "Hr"); eauto.
     iNext. iIntros "Hq".
-    iApply "HΦ". iExists _; iFrame.
+    iApply "HΦ".
+    iExists (Token q); iFrame; iExists _; iFrame.
+    by iAlways; iIntros "$".
   Qed.
 
-  Lemma wp_send_to_nick : ∀ s n m μ,
-    {{{ token s ∗ SendToNick s n {| Shead := m; Stail := μ|} }}}
+  Lemma wp_send_to_nick : ∀ S n m μ,
+    {{{ S ∗ SendToNick S n {| Shead := m; Stail := μ|} }}}
       App (App send_to_nick (of_val n)) (of_val m)
-    {{{ RET UnitV; ∃ s', token s' ∗ SendToNick s' n μ }}}.
+    {{{ RET UnitV; ∃ S', S' ∗ SendToNick S' n μ }}}.
   Proof.
-    iIntros (r n m μ Φ) "[Hr Hrfn] HΦ".
+    iIntros (S n m μ Φ) "[Hs Hrfn] HΦ".
     iApply (wp_bind (fill [AppLCtx _])).
     iApply wp_pure_step_later; trivial.
     iNext. asimpl. iApply wp_value; simpl.
     iApply wp_pure_step_later; trivial.
     iNext. asimpl.
     destruct n; simpl; try done.
+    iDestruct "Hrfn" as (s) "[#HPs Hrfn]".
+    iMod ("HPs" with "Hs") as "Hs".
     rewrite {1}/IO_sequence greatest_fixpoint_unfold.
     iDestruct "Hrfn" as (q) "/= [% Hrfn]".
     iApply (wp_bind (fill [SeqCtx _])).
     iApply (wp_bind (fill [IOLCtx _])).
-    iApply wp_to_read_tag; trivial.
+    iApply wp_to_write_tag; trivial.
     iNext; iIntros "_"; simpl.
-    iApply (wp_petrinet_io with "Hr"); eauto.
+    iApply (wp_petrinet_io with "Hs"); eauto.
     iNext. iIntros "Hq".
     iApply wp_pure_step_later; trivial.
     iNext. iApply wp_value.
-    iApply "HΦ". iExists _; iFrame.
+    iApply "HΦ". iExists (Token q); iFrame; iExists _; iFrame.
+    by iAlways; iIntros "$".
   Qed.
 
   Global Program Instance concrete_nick_comm_prog : abstract_nick_comm_prog :=
@@ -167,16 +179,16 @@ Section conrete_chat_server.
   Program Definition concrete_serveChatRoom :=
     serveChatRoom (BoolV true) (BoolV false).
 
-  Theorem wp_concrete_serverChatRoom r1 r2 s μ1 μ2 :
-    {{{ token r1 ∗ ReceiveFromNick r1 (BoolV true) μ1 ∗
-        token r2 ∗ ReceiveFromNick r2 (BoolV false) μ2 ∗
-        token s ∗ ∀ μ, ⌜interleaving μ1 μ2 μ⌝ →
-                       SendToNicks s (BoolV true) (BoolV false) μ }}}
+  Theorem wp_concrete_serverChatRoom R1 R2 S μ1 μ2 :
+    {{{ R1 ∗ ReceiveFromNick R1 (BoolV true) μ1 ∗
+        R2 ∗ ReceiveFromNick R2 (BoolV false) μ2 ∗
+        S ∗ ∀ μ, ⌜interleaving μ1 μ2 μ⌝ →
+                       SendToNicks S (BoolV true) (BoolV false) μ }}}
       concrete_serveChatRoom
   {{{RET UnitV; False}}}.
   Proof.
     iIntros (Φ) "(Hr1 & Hrf1 & Hr2 & Hrf2 & Hs & Hsnd) HΦ".
-    iApply (wp_serverChatRoom _ _ r1 r2 s with "[-HΦ]"); simpl; eauto.
+    iApply (wp_serverChatRoom _ _ R1 R2 S with "[-HΦ]"); simpl; eauto.
     iFrame.
   Qed.
 
@@ -204,48 +216,66 @@ Inductive chat_server_petri_places :=
 | CHPP_input1 (n : nat)
 | CHPP_input2 (n : nat)
 | CHPP_output
-| CHPP_output1 (n : nat)
-| CHPP_output2 (n : nat).
+| CHPP_output1 (mixer : Stream bool) (n : nat)
+| CHPP_output2 (mixer : Stream bool) (n : nat).
 
 Global Instance chat_server_petri_places_eqdec :
   EqDecision chat_server_petri_places.
-Proof. solve_decision. Qed.
+Proof. intros ??; apply excluded_middle_informative. Qed.
 
 Instance chat_server_petri_placesC : PlacesC :=
   {| Places := chat_server_petri_places |}.
 
-Inductive chat_server_petri_base mixer μ1 μ2 : PetriNet :=
+Inductive chat_server_petri μ1 μ2 : PetriNet :=
 | chat_server_petri_start_split :
-    chat_server_petri_base mixer μ1 μ2 (SplitTr CHPP_Start CHPP_input CHPP_output)
+    chat_server_petri μ1 μ2 (SplitTr CHPP_Start CHPP_input CHPP_output)
 | chat_server_petri_input_split :
-    chat_server_petri_base mixer μ1 μ2
+    chat_server_petri μ1 μ2
                       (SplitTr CHPP_input (CHPP_input1 0) (CHPP_input2 0))
-| chat_server_petri_output_split :
-    chat_server_petri_base mixer μ1 μ2
-                      (SplitTr CHPP_output (CHPP_output1 0) (CHPP_output2 0))
+| chat_server_petri_output_split mixer :
+    chat_server_petri
+      μ1 μ2 (SplitTr CHPP_output (CHPP_output1 mixer 0) (CHPP_output2 mixer 0))
 | chat_server_petri_input1 n :
-    chat_server_petri_base mixer μ1 μ2
+    chat_server_petri μ1 μ2
                       (IOTr (CHPP_input1 n) read_nick1 UnitV (Snth n μ1)
                             (CHPP_input1 (S n)))
 | chat_server_petri_input2 n :
-    chat_server_petri_base mixer μ1 μ2
+    chat_server_petri μ1 μ2
                       (IOTr (CHPP_input2 n) read_nick2 UnitV (Snth n μ2)
                             (CHPP_input2 (S n)))
-| chat_server_petri_output1 n :
-    chat_server_petri_base mixer μ1 μ2
-                      (IOTr (CHPP_output1 n) write_nick1
+| chat_server_petri_output1 mixer n :
+    chat_server_petri μ1 μ2
+                      (IOTr (CHPP_output1 mixer n) write_nick1
                             (Snth n (Smix mixer μ1 μ2))
                             UnitV
-                            (CHPP_output1 (S n)))
-| chat_server_petri_output2 n :
-    chat_server_petri_base mixer μ1 μ2
-                      (IOTr (CHPP_output2 n) write_nick2
+                            (CHPP_output1 mixer (S n)))
+| chat_server_petri_output2 mixer n :
+    chat_server_petri μ1 μ2
+                      (IOTr (CHPP_output2 mixer n) write_nick2
                             (Snth n (Smix mixer μ1 μ2))
                             UnitV
-                            (CHPP_output2 (S n))).
+                            (CHPP_output2 mixer (S n))).
 
-Definition chat_server_petri μ1 μ2 : PetriNet :=
-  λ T, ∃ mixer, chat_server_petri_base mixer μ1 μ2 T.
+Inductive Reachable_Valuation : Valuation → Prop :=
+| ReachableV_Start : Reachable_Valuation (singVAL CHPP_Start)
+| ReachableV_IO :
+    Reachable_Valuation ((singVAL CHPP_input) ⊎ (singVAL CHPP_output))
+| ReachableV_IsO n m :
+    Reachable_Valuation
+      ((singVAL (CHPP_input1 n))
+         ⊎ (singVAL (CHPP_input2 m))
+         ⊎ (singVAL CHPP_output))
+| ReachableV_IOs mixer n m :
+    Reachable_Valuation
+      ((singVAL CHPP_input)
+         ⊎ (singVAL (CHPP_output1 mixer n))
+         ⊎ (singVAL (CHPP_output2 mixer m)))
+| ReachableV_IsOs mixer n1 m1 n2 m2 :
+    Reachable_Valuation
+      ((singVAL (CHPP_input1 n1))
+         ⊎ (singVAL (CHPP_input2 m1))
+         ⊎ (singVAL (CHPP_output1 mixer n2))
+         ⊎ (singVAL (CHPP_output2 mixer m2))).
 
 (* Lemma chat_server_petri_det_io mixer μ1 μ2 : *)
 (*   (∀ p t v v' q, *)
@@ -280,29 +310,130 @@ Definition chat_server_petri μ1 μ2 : PetriNet :=
 (* Definition chat_server_petri_start_val := *)
 (*   λ p, match p with CHPP_Start => 1 | _ => 0 end. *)
 
-(* correct the statement, p must be reachable from start! *)
-Lemma chat_server_petri_ResultDet μ1 μ2 p :
-  ResultDet (Traces (chat_server_petri μ1 μ2) p).
+Lemma singVAL_eq p q V : singVAL p ⊎ V = singVAL q → p = q ∧ V = (λ x, 0).
 Proof.
-  (* intros t v v' v'' τ τ' τ'' Hτ. *)
-  (* remember (τ ++ (t, v, v') :: τ') as io. *)
-  (* revert τ t v v' v'' τ' Heqio. *)
-  (* induction Hτ as [| ? ? ? ? ? ? ? Hτio | | |] => τ1 t1 v1 v1' v1'' τ1' Heqio Hτ''. *)
-  (* - by destruct τ1. *)
-  (* - inversion Hτ''. *)
-  (*   + by destruct τ1. *)
-  (*   + destruct τ1 as [|[[? ?] ?] τ1]; simpl in *; inversion Heqio; simplify_eq. *)
-  (*     * admit. *)
-  (*     *  *)
+  intros Heq.
+  split.
+  - pose proof (equal_f Heq p) as Heq'.
+    revert Heq'. rewrite /singVAL /ValPlus /=.
+    repeat destruct decide; done.
+  - extensionality z.
+    pose proof (equal_f Heq z) as Heq'.
+    pose proof (equal_f Heq p) as Heq''.
+    revert Heq' Heq''. rewrite /singVAL /ValPlus /=.
+    repeat destruct decide; subst; auto with omega; try done.
+Qed.
+
+Lemma singVAL_eq21 p1 p2 q V :
+  p1 ≠ p2 → singVAL p1 ⊎ singVAL p2 = singVAL q ⊎ V → q = p1 ∨ q = p2.
+Proof.
+  intros ? Heq.
+  pose proof (equal_f Heq q) as Heq'.
+  revert Heq'. rewrite /singVAL /ValPlus /=.
+  repeat destruct decide; simplify_eq; eauto with lia.
+Qed.
+
+Lemma singVAL_eq12 p q1 q2 V : ¬ singVAL p = singVAL q1 ⊎ singVAL q2 ⊎ V.
+Proof.
+  intros Heq.
+  pose proof (equal_f Heq p) as Heq'.
+  pose proof (equal_f Heq q1) as Heq''.
+  pose proof (equal_f Heq q2) as Heq'''.
+  revert Heq' Heq'' Heq'''. rewrite /singVAL /ValPlus /=.
+  repeat (destruct decide; try done); simplify_eq; eauto with lia.
+Qed.
+
+Lemma singVAL_eq22 p1 p2 q1 q2 V :
+  p1 ≠ p2 →
+  singVAL p1 ⊎ singVAL p2 = singVAL q1 ⊎ singVAL q2 ⊎ V →
+  q1 = p1 ∧ q2 = p2 ∨ q1 = p2 ∧ q2 = p1.
+Proof.
+  intros ? Heq.
+  pose proof (equal_f Heq p1) as Heq1.
+  pose proof (equal_f Heq q2) as Heq2.
+  pose proof (equal_f Heq q1) as Heq3.
+  pose proof (equal_f Heq q2) as Heq4.
+  revert Heq1 Heq2 Heq3 Heq4. rewrite /singVAL /ValPlus /=.
+  repeat (destruct decide; try done); simplify_eq; eauto with lia.
+Qed.
+
+(* Lemma singVAL_eq32 p1 p2 p3 q1 q2 V : *)
+(*   p1 ≠ p2 → *)
+(*   singVAL p1 ⊎ singVAL p2 ⊎ singVAL p3 = singVAL q1 ⊎ singVAL q2 ⊎ V → *)
+(*   (q1 = p1 ∧ q2 = p2) ∨ (q1 = p2 ∧ q2 = p1) ∨ *)
+(*   (q1 = p1 ∧ q2 = p2). *)
+(* Proof. *)
+(*   intros ? Heq. *)
+(*   pose proof (equal_f Heq p1) as Heq1. *)
+(*   pose proof (equal_f Heq q2) as Heq2. *)
+(*   pose proof (equal_f Heq q1) as Heq3. *)
+(*   pose proof (equal_f Heq q2) as Heq4. *)
+(*   revert Heq1 Heq2 Heq3 Heq4. rewrite /singVAL /ValPlus /=. *)
+(*   repeat (destruct decide; try done); simplify_eq; eauto with lia. *)
+(* Qed. *)
+
+
+(* There are so many cases that we need to consider we just admit them
+here. There must be an easier way via some more disciplined lemma to
+prove result-deterministicness that does not involve so many case
+analysis over the transitions and valuations. *)
+(* admitted cases below are intuitively easy! *)
+Lemma chat_server_petri_ResultDet μ1 μ2 V :
+  Reachable_Valuation V →
+  ResultDet (Traces (chat_server_petri μ1 μ2) V).
+Proof.
+  intros HV t v v' v'' τ τ' τ'' Hτ.
+  remember (τ ++ (t, v, v') :: τ') as io.
+  revert HV τ t v v' v'' τ' Heqio.
+  induction Hτ as [| ? ? ? ? ? ? ? Hτio | | |] => HV τ1 t1 v1 v1' v1'' τ1' Heqio Hτ''.
+  - by destruct τ1.
+  - inversion HV.
+    + edestruct singVAL_eq; eauto; subst.
+      match goal with
+      | H : chat_server_petri _ _ _ |- _ => inversion H
+      end.
+    + edestruct (singVAL_eq21); eauto; try done; simplify_eq;
+        match goal with
+        | H : chat_server_petri _ _ _ |- _ => inversion H
+        end.
+    + admit.
+    + admit.
+    + admit.
+  - match goal with
+    | H : chat_server_petri _ _ (SplitTr ?p _ _) |- _ =>
+      destruct p; inversion H; simplify_eq
+    end.
+    + inversion HV.
+      * admit.
+      * edestruct singVAL_eq21; eauto; try done.
+      * admit.
+      * admit.
+      * admit.
+    + admit.
+    + inversion HV.
+      * edestruct singVAL_eq; eauto; try done.
+      * edestruct singVAL_eq21; eauto; try done.
+        admit.
+      * admit.
+      * admit.
+      * admit.
+  - match goal with
+        | H : chat_server_petri _ _ (JoinTr ?p _ _) |- _ =>
+          destruct p; inversion H
+        end.
+  - match goal with
+    | H : chat_server_petri _ _ (NoOpTr ?p _) |- _ =>
+      destruct p; inversion H
+    end.
 Admitted.
 
-Lemma Recive_from_nick (b : bool) `{inG Σ (authUR (ofe_funUR (λ _ : Places, natUR)))}
-      γ μ1 μ2 :
-  let _ := {| γPN := γ; ThePetriNet := chat_server_petri μ1 μ2 |}in
-  (ReceiveFromNick (if b then (CHPP_input1 0) else (CHPP_input2 0))
+Lemma Recive_from_nick (b : bool)
+      `{heapIG Σ} `{inG Σ (authUR (ofe_funUR (λ _ : Places, natUR)))} γ μ1 μ2 :
+  let _ := {| γPN := γ; ThePetriNet := chat_server_petri μ1 μ2 |} in
+  (ReceiveFromNick (if b then Token (CHPP_input1 0) else Token (CHPP_input2 0))
                    (BoolV b) (if b then μ1 else μ2))%I.
 Proof.
-  pose ({| γPN := γ; PNI_exclG := H;
+  pose ({| γPN := γ; PNI_exclG := _;
            ThePetriNet := chat_server_petri μ1 μ2 |}).
   set (Φ := (λ pμ : @place_stream chat_server_petri_placesC,
                       ∃ n, ⌜pμ.1 = (if b then CHPP_input1 n else CHPP_input2 n)
@@ -311,36 +442,46 @@ Proof.
   assert (NonExpansive Φ).
   { by intros n [? ?] [? ?] [?%leibniz_equiv ?%leibniz_equiv];
       simpl in *; subst. }
+  iExists (if b then (CHPP_input1 0) else (CHPP_input2 0)); simpl.
+  iSplit.
+  { by destruct b; iIntros "!# $". }
   iApply (greatest_fixpoint_coind _ Φ); simpl; eauto.
   iAlways. iIntros ([? ?]); iDestruct 1 as %[n [Hn Hμ]]; simpl in *; subst.
   rewrite /IO_pre_sequence.
   iExists (if b then CHPP_input1 (S n) else CHPP_input2 (S n)); iSplit; simpl.
-  + iPureIntro. rewrite Snth_Sdrop; destruct b; exists (Sconst true); constructor.
+  + iPureIntro. rewrite Snth_Sdrop; destruct b; econstructor.
   + iExists (S n); iPureIntro; split; simpl; auto.
 Qed.
 
-Lemma Send_to_nick (b : bool) `{inG Σ (authUR (ofe_funUR (λ _ : Places, natUR)))}
+Lemma Send_to_nick (b : bool) mixer
+      `{heapIG Σ} `{inG Σ (authUR (ofe_funUR (λ _ : Places, natUR)))}
       γ μ1 μ2 μ :
-  interleaving μ1 μ2 μ →
+  Smix mixer μ1 μ2 = μ →
   let _ := {| γPN := γ; ThePetriNet := chat_server_petri μ1 μ2 |}in
-  (SendToNick (if b then (CHPP_output1 0) else (CHPP_output2 0)) (BoolV b) μ)%I.
+  (SendToNick (if b then Token (CHPP_output1 mixer 0) else
+                 Token (CHPP_output2 mixer 0)) (BoolV b) μ)%I.
 Proof.
-  pose ({| γPN := γ; PNI_exclG := H;
+  pose ({| γPN := γ; PNI_exclG := _;
            ThePetriNet := chat_server_petri μ1 μ2 |}).
   set (Φ := (λ pμ : @place_stream chat_server_petri_placesC,
-                      ∃ n, ⌜pμ.1 = (if b then CHPP_output1 n else CHPP_output2 n)
+                      ∃ n, ⌜pμ.1 = (if b then CHPP_output1 mixer n else
+                                      CHPP_output2 mixer n)
                            ∧ pμ.2 = Sdrop n μ⌝)%I
             : place_stream → iProp Σ).
   assert (NonExpansive Φ).
   { by intros n [? ?] [? ?] [?%leibniz_equiv ?%leibniz_equiv];
       simpl in *; subst. }
   intros Hinr; simpl.
+  iExists (if b then (CHPP_output1 mixer 0) else (CHPP_output2 mixer 0)); simpl.
+  iSplit.
+  { by destruct b; iIntros "!# $". }
   iApply (greatest_fixpoint_coind _ Φ); simpl; eauto.
   iAlways. iIntros ([? ?]); iDestruct 1 as %[n [Hn Hμ]]; simpl in *; subst.
   rewrite /IO_pre_sequence.
-  iExists (if b then CHPP_output1 (S n) else CHPP_output2 (S n)); iSplit; simpl.
-  + iPureIntro. rewrite Snth_Sdrop. destruct Hinr as [mixer <-].
-    destruct b; exists mixer; econstructor.
+  iExists (if b then CHPP_output1 mixer (S n) else CHPP_output2 mixer (S n));
+    iSplit; simpl.
+  + iPureIntro. rewrite Snth_Sdrop.
+    destruct b; econstructor.
   + iExists (S n); iPureIntro; split; simpl; auto.
 Qed.
 
@@ -365,29 +506,32 @@ Proof.
   iModIntro. iExists _. pose (make_heapIG γio). iFrame.
   iMod (PetriNetInv_alloc with "HOI") as (γpn) "[#HPi HOV]".
   { apply chat_server_petri_ResultDet. }
-  pose ({| PNI_exclG := _; γPN := γpn; ThePetriNet := chat_server_petri μ1 μ2|})
-    as PN.
+  pose ({| γPN := γpn; ThePetriNet := chat_server_petri μ1 μ2|}) as PN.
   iModIntro. iExists PN.
   iAssert (@Token chat_server_petri_placesC _ _ _ CHPP_Start) with "[$HOV]"
     as "HOS"; first done.
   iMod (petrinet_split with "[HOS]") as "[HI HO]"; [| by iFrame |].
-  { exists (Sconst true); apply chat_server_petri_start_split. }
+  { apply chat_server_petri_start_split. }
   iMod (petrinet_split with "[HI]") as "[HI1 HI2]"; [| by iFrame |].
-  { exists (Sconst true); apply chat_server_petri_input_split. }
-  iPoseProof (Recive_from_nick true γpn μ1 μ2) as "HRFN1".
-  iPoseProof (Recive_from_nick false γpn μ1 μ2) as "HRFN2".
-  iApply (@wp_concrete_serverChatRoom
-            _ _ chat_server_petri_placesC _ _
-            (CHPP_input1 0) (CHPP_input2 0) CHPP_output μ1 μ2 with "[-]");
+  { apply chat_server_petri_input_split. }
+  iPoseProof (Recive_from_nick true γpn μ1 μ2) as (r) "[#Hr1 HRFN1]".
+  iPoseProof (Recive_from_nick false γpn μ1 μ2) as (s) "[#Hr2 HRFN2]".
+  iApply (wp_concrete_serverChatRoom
+            (@Token _ _ _ PN (CHPP_input1 0)) (@Token _ _ _ PN (CHPP_input2 0))
+            (@Token _ _ _ PN CHPP_output) μ1 μ2 with "[-]");
     last done.
-  iFrame; iFrame "#".
-  iIntros (μ Hintr).
-  iExists _, _; simpl.
-  iSplit.
-  { iPureIntro. eexists (Sconst true); econstructor. }
+  iFrame.
   iSplitL.
-  by iApply (Send_to_nick true).
-  by iApply (Send_to_nick false).
+  { iExists _; iFrame "#". }
+  iSplitL.
+  { iExists _; iFrame "#". }
+  iIntros (μ [mixer <-]).
+  iExists (Token _), (Token _); simpl.
+  iSplit.
+  { iApply petrinet_split. apply (chat_server_petri_output_split _ _ mixer). }
+  iSplitL.
+  { by iApply (Send_to_nick true). }
+  { by iApply (Send_to_nick false). }
 Qed.
 
 Theorem concrete_serverChatRoom_safe :
@@ -413,10 +557,10 @@ Proof.
     apply leibniz_equiv in HM; subst.
     pose (#[IoΣ; petrinetΣ; channelΣ]) as Σ.
     apply (adequacy Σ _ ((λ _, False))%I).
-    { admit. }
+    { apply Traces_prefix_closed. }
     intros Hig.
     iIntros "".
     iMod (wp_closed_concrete_serverChatRoom μ1 μ2) as (γio) "Hlm".
     iMod ("Hlm") as (HIG) "[HFIO HWP]".
     iModIntro; iExists _; iFrame.
-Admitted.
+Qed.
